Port multistep stuff from Simple into SystemF

proof/SystemF/EsJudge.v
@@ -33,5 +33,123 @@ Inductive STEP : exp -> exp -> Prop :=
     ,  STEP x1 x1'
     -> STEP (XAPP x1 t2) (XAPP x1' t2).
 
+Hint Constructors STEP.
 
-        
+
+(* Multi-step evaluation *******************************************
+   A sequence of small step transitions.
+   As opposed to STEPSL, this version has an append constructor
+   ESAppend that makes it easy to join two evaluations together.
+   We use this when converting big-step evaluations to small-step.
+ *)
+Inductive STEPS : exp -> exp -> Prop :=
+
+ (* After no steps, we get the same exp.
+    We need this constructor to match the EVDone constructor
+    in the big-step evaluation, so we can convert between big-step
+    and multi-step evaluations. *)
+ | ESNone
+   :  forall x1
+   ,  STEPS x1 x1
+
+ (* Take a single step. *)
+ | ESStep
+   :  forall x1 x2
+   ,  STEP  x1 x2
+   -> STEPS x1 x2
+
+ (* Combine two evaluations into a third. *)
+ | ESAppend
+   :  forall x1 x2 x3
+   ,  STEPS x1 x2 -> STEPS x2 x3
+   -> STEPS x1 x3.
+
+Hint Constructors STEPS.
+
+
+(* Context lemmas ***************************************************
+   These help when proving something about a reduction in a given
+   context. They're all trivial.
+ *)
+Lemma steps_app1
+ :  forall x1 x1' x2
+ ,  STEPS x1 x1'
+ -> STEPS (XApp x1 x2) (XApp x1' x2).
+Proof.
+ intros. induction H; eauto.
+Qed.
+Hint Resolve steps_app1.
+
+
+Lemma steps_app2
+ :  forall v1 x2 x2'
+ ,  value v1 
+ -> STEPS x2 x2'
+ -> STEPS (XApp v1 x2) (XApp v1 x2').
+Proof.
+ intros. induction H0; eauto.
+Qed.
+Hint Resolve steps_app2.
+
+
+Lemma steps_APP1
+ :  forall x1 x1' t2
+ ,  STEPS x1 x1'
+ -> STEPS (XAPP x1 t2) (XAPP x1' t2).
+Proof.
+ intros. induction H; eauto.
+Qed.
+
+
+(* Left linearised multi-step evaluation ****************************
+   As opposed to STEPS, this version provides a single step at a time
+   and does not have an append constructor. This is convenient
+   when converting a small-step evaluations to big-step, via the
+   eval_expansion lemma.
+ *)
+Inductive STEPSL : exp -> exp -> Prop :=
+
+ | ESLNone 
+   : forall x1
+   , STEPSL x1 x1
+
+ | ESLCons
+   :  forall x1 x2 x3
+   ,  STEP   x1 x2 -> STEPSL x2 x3 
+   -> STEPSL x1 x3.
+
+Hint Constructors STEPSL.
+
+
+(* Transitivity of left linearised multi-step evaluation.
+   We use this when "flattening" a big step evaluation to the
+   small step one.
+ *)
+Lemma stepsl_trans
+ :  forall x1 x2 x3
+ ,  STEPSL x1 x2 -> STEPSL x2 x3
+ -> STEPSL x1 x3.
+Proof.
+ intros.
+ induction H.
+  eauto.
+  eapply ESLCons. eauto. eauto.
+Qed.
+
+
+(* Linearise a regular multi-step evaluation.
+   This flattens out all the append constructors, leaving us with
+   a list of individual transitions. 
+ *)
+Lemma stepsl_of_steps
+ :  forall x1 x2
+ ,  STEPS  x1 x2
+ -> STEPSL x1 x2.
+Proof. 
+ intros.
+ induction H.
+  auto.
+  eauto.
+  eapply stepsl_trans; eauto.
+Qed.
+
